Auto/Lib/HEqExtra.lean
@@ -1,3 +1,5 @@
+namespace Auto
+
 def HEq.tyEq {α β : Sort u} (x : α) (y : β) (H : HEq x y) : α = β :=
   match β, y, H with
   | .(α), .(x), HEq.refl _ => Eq.refl _
@@ -11,6 +13,14 @@ def HEq.funext {γ : Sort u} {α β : γ → Sort v}
       match xyEq with
       | Eq.refl _ => HEq.refl _) (_root_.funext (fun u => HEq.tyEq _ _ (H u)))
 
+theorem congr_heq {α β γ : Sort _} {f : α → γ} {g : β → γ} {x : α} {y : β}
+    (h₁ : HEq f g) (h₂ : HEq x y) : f x = g y := by
+  cases h₂; cases h₁; rfl
+
+theorem congr_arg_heq {α} {β : α → Sort _} (f : ∀ a, β a) :
+    ∀ {a₁ a₂ : α}, a₁ = a₂ → HEq (f a₁) (f a₂)
+  | _, _, rfl => HEq.rfl
+
 theorem heq_of_eqRec_eq' {motive : γ → Sort u} {α β : γ} (h₁ : α = β)
   (a : motive α) : HEq a (@Eq.rec γ α (fun α _ => motive α) a β h₁) := by
   subst h₁
@@ -22,3 +32,5 @@ theorem congr_arg₂_heq {β : α → Sort _} (γ : ∀ (a : α), β a → Sort 
   subst H₁
   cases H₂
   apply HEq.refl
+
+end Auto
